iris/ProofSyscall.v
@@ -3348,18 +3348,20 @@ Section SyscallArms.
   Qed.
 
   Lemma sysc_dep_mkdir (U : ustate) (sts : list fdstate) (gn : gname) (cs : gset gname)
-      (pid : mword 32) (f : sfam) :
+      (pid : mword 32) (f : sfam) (v0 : mword 64) :
     sysc_num (us_V U) = 20 ->
+    pv_tf (us_V U) !! tf_arg_idx 0 = Some v0 ->
     sysc_sys_in U sts gn cs pid f -∗
-    mkdir_au_pre (fs_gamma_L fsc_fs) fsc_fs (pv_cwi (us_V U))
+    mkdir_au_at (fs_gamma_L fsc_fs) fsc_fs (pv_cwi (us_V U)) (us_M U) v0
       (df_P f) (df_Pmiss f) (df_Farm f) (df_Fdots f) (df_Fun f)
       (df_Fok f) (df_Fex f).
   Proof.
-    intros Hn. iIntros "H".
+    intros Hn Hv0. iIntros "H".
     iDestruct (sysc_sys_in_at U sts gn cs pid f 20 Hn ltac:(vm_compute; discriminate)
                  ltac:(vm_compute; discriminate) with "H") as "H".
     iDestruct (sbundle_at_mkdir_elim uslot f _ with "H") as "H".
-    rewrite /uvis_of. cbn [uvis_cwd]. iExact "H".
+    rewrite /uvis_of /tf_w. cbn [uvis_cwd uvis_tf uvis_M].
+    rewrite (list_lookup_total_correct _ _ _ Hv0). iExact "H".
   Qed.
 
   (* ================================================================== *)
@@ -3579,20 +3581,22 @@ Section SyscallArms.
   Qed.
 
   Lemma sysc_out_mkdir (U : ustate) (sts : list fdstate) (gn : gname) (cs : gset gname)
-      (pid : mword 32) (f : sfam)
+      (pid : mword 32) (f : sfam) (v0 : mword 64)
       (r : mword 64) (M' : gmap Z (bv 8)) (sts' : list fdstate) (cw' : Z) (cs' : gset gname) :
     sysc_num (us_V U) = 20 ->
+    pv_tf (us_V U) !! tf_arg_idx 0 = Some v0 ->
     mkdir_arms (fs_gamma_L fsc_fs) fsc_fs (pv_cwi (us_V U))
       (df_P f) (df_Pmiss f) (df_Farm f) (df_Fdots f) (df_Fun f)
-      (df_Fok f) (df_Fex f) r -∗
+      (df_Fok f) (df_Fex f) (us_M U) v0 r -∗
     sysc_sys_out U sts gn cs pid f r M' sts' cw' cs'.
   Proof.
-    intros Hn. iIntros "H".
+    intros Hn Hv0. iIntros "H".
     iApply (sysc_sys_out_at U sts gn cs pid f r M' sts' cw' cs' 20 Hn
               ltac:(vm_compute; discriminate)
               ltac:(vm_compute; discriminate)).
     iApply (spost_at_mkdir_intro uslot f (uvis_of U sts gn cs pid) r M' sts' cw' cs').
-    rewrite /uvis_of. cbn [uvis_cwd]. iExact "H".
+    rewrite /uvis_of /tf_w. cbn [uvis_cwd uvis_tf uvis_M].
+    rewrite (list_lookup_total_correct _ _ _ Hv0). iExact "H".
   Qed.
 
   Lemma sysc_exec_in_open (U : ustate) (sts : list fdstate) (gn : gname) (cs : gset gname)
@@ -7080,8 +7084,8 @@ Section SyscallArms.
                     Hgen Hdevi Hgeom Hdlock Hbs Hit Hitinv Hesc Hsl2 Hireg
                     Hropen Hsbn Hisp Hsbs Hbmp Hbmr Hkalloc Hprocs Hir Hpriv
                     [Hxin]").
-    { iApply (sysc_dep_mkdir U sts gn cs pid fdep ltac:(rewrite Hnum; reflexivity)
-                with "Hxin"). }
+    { iApply (sysc_dep_mkdir U sts gn cs pid fdep v0
+                ltac:(rewrite Hnum; reflexivity) Hv0 with "Hxin"). }
     iIntros (CIDy Hsy mf ns' P')
       "%Hcs %Hextz Hcg Hcpu _ _ Hpc Hbs _ _ _ _ %Hns Hir Hpriv %Hret0 Harms".
     (* [Hextz] is the SIZED extension the callee reports, and it is what
@@ -7148,8 +7152,8 @@ Section SyscallArms.
     (* ...and wait answers nothing here either *)
     { iApply sysc_wait_out_ne. unfold UsysMemOk.USYS_wait in *; lia. }
     iApply (sysc_exec_out_ne _ _ _ _ _ _ _ _ (sysc_num_ne7 _ _ Hnum eq_refl)).
-    iApply (sysc_out_mkdir U sts gn cs pid fdep (mf !!! Regidx Ra0) _ _ _ _
-              ltac:(rewrite Hnum; reflexivity) with "Harms").
+    iApply (sysc_out_mkdir U sts gn cs pid fdep v0 (mf !!! Regidx Ra0) _ _ _ _
+              ltac:(rewrite Hnum; reflexivity) Hv0 with "Harms").
   Qed.
 
   (* ------------------------------------------------------------------- *)
